theories/zoo_persistent/pqueue.v
@@ -56,9 +56,9 @@ Section zoo_G.
   Proof.
     iIntros "%Φ (%front & %back & (-> & ->)) HΦ".
     wp_rec.
-    wp_smart_apply (lst_is_empty_spec with "[//]") as "_".
+    wp_smart_apply (lst_is_empty_spec with "[//]") as "_"; first done.
     destruct front as [| v front]; wp_pures.
-    - wp_apply (lst_is_empty_spec with "[//]") as "_".
+    - wp_apply (lst_is_empty_spec with "[//]") as "_"; first done.
       erewrite bool_decide_ext by apply reverse_nil_iff. iSteps.
     - rewrite bool_decide_eq_false_2 //. iSteps.
   Qed.
@@ -99,7 +99,7 @@ Section zoo_G.
     iIntros "%Φ (%front & %back & (-> & ->)) HΦ".
     wp_rec.
     destruct front as [| v front]; wp_pures.
-    - wp_apply (lst_rev_spec with "[//]") as "%front ->".
+    - wp_apply (lst_rev_spec with "[//]") as "%front ->"; first done.
       destruct (rev_elim back) as [-> | (back' & v & ->)].
       + wp_pures.
         iApply ("HΦ" $! None with "[//]").
